crypto_hst/ec/Hacl.EC.Curve25519.Bignum.fst
@@ -229,7 +229,7 @@ let fdifference a b =
   push_frame ();
   (* let h0 = HST.get() in *)
   (* standardized_eq_norm h0 a; standardized_eq_norm h0 b; *)
-  let b' = create (Hacl.Cast.uint64_to_sint64 0uL) nlength in
+  let b' = create (Hacl.Cast.uint64_to_sint64 0uL) 5ul in
   let tmp = create (Hacl.Cast.uint64_to_sint128 0uL) (U32 (2ul *^ nlength -^ 1ul)) in
   blit b 0ul b' 0ul nlength;
   (* let b' = Bigint.copy b in  *)
